ver2/optimizations/and_and1.v
@@ -1,0 +1,367 @@
+Require Import bbv.Word.
+Require Import Nat. 
+Require Import Coq.NArith.NArith.
+Require Import Coq.Bool.Bool.
+
+Require Import Coq.Logic.FunctionalExtensionality.
+
+Require Import FORVES.constants.
+Import Constants.
+
+Require Import FORVES.symbolic_state.
+Import SymbolicState.
+
+Require Import FORVES.symbolic_state_eval.
+Import SymbolicStateEval.
+
+Require Import FORVES.symbolic_state_cmp.
+Import SymbolicStateCmp.
+
+Require Import FORVES.valid_symbolic_state.
+Import ValidSymbolicState.
+
+Require Import FORVES.execution_state.
+Import ExecutionState.
+
+Require Import FORVES.stack_operation_instructions.
+Import StackOpInstrs.
+
+Require Import FORVES.program.
+Import Program.
+
+Require Import FORVES.symbolic_state_cmp_impl.
+Import SymbolicStateCmpImpl.
+
+Require Import FORVES.symbolic_state_eval_facts.
+Import SymbolicStateEvalFacts.
+
+Require Import FORVES.valid_symbolic_state.
+Import ValidSymbolicState.
+
+Require Import FORVES.misc.
+Import Misc.
+
+Require Import FORVES.eval_common.
+Import EvalCommon.
+
+Require Import FORVES.concrete_interpreter.
+Import ConcreteInterpreter.
+
+Require Import FORVES.optimizations_def.
+Import Optimizations_Def.
+
+Require Import FORVES.optimizations_common.
+Import Optimizations_Common.
+
+Require Import List.
+Import ListNotations.
+
+
+Module Opt_and_and1.
+
+(* sv1 sv2 maxidx1 sb1 maxid2 sb2 instk_height ops -> bool *)
+Definition sstack_val_cmp_t := sstack_val -> sstack_val -> nat -> sbindings -> nat -> sbindings -> nat -> stack_op_instr_map -> bool.
+
+(* AND(X,AND(X,Y)) = AND(X,Y)
+   AND(X,AND(Y,X)) = AND(X,Y)
+ *)
+Definition optimize_and_and1_sbinding : opt_smap_value_type := 
+fun (val: smap_value) =>
+fun (fcmp: sstack_val_cmp_t) =>
+fun (sb: sbindings) =>
+fun (maxid: nat) =>
+fun (instk_height: nat) =>
+fun (ops: stack_op_instr_map) => 
+match val with
+| SymOp AND [arg1;arg2] => 
+  match follow_in_smap arg2 maxid sb with
+  | Some (FollowSmapVal (SymOp AND [arg21;arg22]) idx' sb') => 
+      if fcmp arg1 arg21 maxid sb idx' sb' instk_height ops then 
+        (SymOp AND [arg1;arg22], true)
+      else if fcmp arg1 arg22 maxid sb idx' sb' instk_height ops then 
+        (SymOp AND [arg1;arg21], true)
+      else 
+        (val, false)
+  | _ => (val, false)
+  end
+| _ => (val, false)
+end.
+
+
+Lemma wand_x_x: forall (x: EVMWord),
+wand x x = x.
+Proof.
+induction x as [|b n x' IH].
+- reflexivity.
+- unfold wand. simpl. fold wand.
+  rewrite -> andb_diag.
+  rewrite -> IH.
+  reflexivity.
+Qed.
+
+
+Lemma wand_wand1_1: forall (x y: EVMWord),
+wand x (wand x y) = wand x y.
+Proof.
+intros x y.
+rewrite -> wand_assoc.
+rewrite -> wand_x_x.
+reflexivity.
+Qed.
+
+Lemma wand_wand1_2: forall (x y: EVMWord),
+wand x (wand y x) = wand x y.
+Proof.
+intros x y.
+rewrite -> wand_comm.
+rewrite <- wand_assoc.
+rewrite -> wand_x_x.
+rewrite -> wand_comm.
+reflexivity.
+Qed.
+
+
+Lemma optimize_and_and1_sbinding_smapv_valid:
+opt_smapv_valid_snd optimize_and_and1_sbinding.
+Proof.
+Admitted.
+(*
+unfold opt_smapv_valid_snd.
+intros instk_height n ops fcmp sb val val' flag.
+intros Hvalid_smapv_val Hvalid Hoptm_sbinding.
+unfold optimize_not_not_sbinding in Hoptm_sbinding.
+destruct (val) as [basicv|pushtagv|label args|offset smem|key sstrg|
+  offset size smem] eqn: eq_val; 
+  try inject_rw Hoptm_sbinding eq_val'.
+destruct label eqn: eq_label; try try inject_rw Hoptm_sbinding eq_val'.
+destruct args as [|arg1 r1] eqn: eq_args; try inject_rw Hoptm_sbinding eq_val'.
+destruct r1; try inject_rw Hoptm_sbinding eq_val'.
+destruct (follow_to_op arg1 n sb) as [fsmv|] eqn: eq_follow1;
+  try inject_rw Hoptm_sbinding eq_val'.
+destruct fsmv as [smv idx' sb'] eqn: eq_fsmv.
+destruct smv as [x1|x2|label2 args2|x4|x5|x6] eqn: eq_smv;
+  try inject_rw Hoptm_sbinding eq_val'.
+destruct label2 eqn: eq_label2; try inject_rw Hoptm_sbinding eq_val'.
+destruct args2 as [|arg2 r2] eqn: eq_args2; try inject_rw Hoptm_sbinding eq_val'.
+destruct r2 as [|x1] eqn: eq_r2; try inject_rw Hoptm_sbinding eq_val'.
+injection Hoptm_sbinding as eq_val' _.
+rewrite <- eq_val'.
+unfold valid_stack_op_instr in Hvalid_smapv_val.
+unfold valid_smap_value in Hvalid_smapv_val.
+unfold valid_stack_op_instr in Hvalid_smapv_val.
+destruct (ops NOT) as [nargs f Hcomm Hctx_indep] eqn: eq_ops.
+destruct Hvalid_smapv_val as [eq_len eq_valid_args1].
+simpl in eq_valid_args1.
+destruct eq_valid_args1 as [eq_valid_arg1 _].
+simpl.
+unfold follow_to_op in eq_follow1.
+destruct (follow_in_smap arg1 n sb) as [fsmv1|] eqn: eq_follow_arg1;
+  try discriminate.
+destruct fsmv1  as [smv1 idx1 sb1] eqn: eq_fsmv1.
+destruct smv1 as [x1|x2|op1 args1|x4|x5|x6] eqn: eq_smv1; try discriminate.
+injection eq_follow1 as eq_op1 eq_args1 eq_idx1 eq_sb1.
+rewrite -> eq_op1 in eq_follow_arg1.
+rewrite -> eq_args1 in eq_follow_arg1.
+rewrite -> eq_idx1 in eq_follow_arg1.
+rewrite -> eq_sb1 in eq_follow_arg1.
+pose proof (valid_follow_in_smap sb arg1 instk_height n ops
+  (SymOp NOT [arg2]) idx' sb' eq_valid_arg1 Hvalid eq_follow_arg1) 
+  as Hnew_valid.
+destruct Hnew_valid as [Hvalid_smap_idx' [Hvalid_sb' Himp]].
+assert (not_basic_value_smv (SymOp NOT [arg2]) = true) as not_basic_not_arg2.
+- intuition.
+- apply Himp in not_basic_not_arg2 as n_gt_idx'.
+  simpl in Hvalid_smap_idx'.
+  unfold valid_stack_op_instr in Hvalid_smap_idx'.
+  rewrite -> eq_ops in Hvalid_smap_idx'.
+  simpl in Hvalid_smap_idx'.
+  destruct Hvalid_smap_idx' as [_ [Hvalid_sstack_value_arg2_idx' _]].
+  apply valid_sstack_value_gt with (n:=idx'); try assumption.
+Qed.
+*)
+
+Lemma evm_stack_opm_AND:
+evm_stack_opm AND = OpImp 2 evm_and (Some and_comm) (Some and_ctx_ind).
+Proof.
+reflexivity.
+Qed.
+
+Lemma lenght2: forall {T: Type} (x y: T), (length [x; y] =? 2) = true.
+Proof.
+intros T x y.
+reflexivity.
+Qed.
+
+
+Lemma optimize_and_and1_sbinding_snd:
+opt_sbinding_snd optimize_and_and1_sbinding.
+Proof.
+unfold opt_sbinding_snd.
+intros val val' fcmp sb maxidx instk_height idx flag Hsafe_sstack_val_cmp
+  Hvalid Hoptm_sbinding.
+split.
+- (* valid_sbindings *)
+  apply valid_bindings_snd_opt with (val:=val)(opt:=optimize_and_and1_sbinding)
+    (fcmp:=fcmp)(flag:=flag); try assumption.
+  apply optimize_and_and1_sbinding_smapv_valid. 
+
+- (* evaluation is preserved *) 
+  intros stk mem strg ctx v Hlen Heval_orig.
+  unfold optimize_and_and1_sbinding in Hoptm_sbinding.
+  destruct val as [vv|vv|label args|offset smem|key sstrg|offset seze smem]
+    eqn: eq_val; try inject_rw Hoptm_sbinding eq_val'.
+  (* SymOp label args *)
+  destruct label eqn: eq_label; try inject_rw Hoptm_sbinding eq_val'.
+  destruct args as [|arg1 r1] eqn: eq_args; 
+    try inject_rw Hoptm_sbinding eq_val'.
+  destruct r1 as [|arg2 r2]; try inject_rw Hoptm_sbinding eq_val'.
+  destruct r2 as [|arg3 r3]; try inject_rw Hoptm_sbinding eq_val'.
+  destruct (follow_in_smap arg2 idx sb) as [fsmv|] eqn: eq_follow_arg2;
+    try inject_rw Hoptm_sbinding eq_val'.
+  destruct fsmv as [smv idx' sb'] eqn: eq_fsmv.
+  destruct smv as [_1|_2|label2 args2|_4|_5|_6] eqn: eq_smv;
+    try inject_rw Hoptm_sbinding eq_val'.
+  destruct label2 eqn: eq_label2; try inject_rw Hoptm_sbinding eq_val'.
+  destruct args2 as [|arg21 r21]; try inject_rw Hoptm_sbinding eq_val'.
+  destruct r21 as [|arg22 r22]; try inject_rw Hoptm_sbinding eq_val'.
+  destruct r22; try inject_rw Hoptm_sbinding eq_val'.
+  
+  assert (Heval_orig_copy := Heval_orig).
+  unfold eval_sstack_val in Heval_orig. simpl in Heval_orig.
+  rewrite -> PeanoNat.Nat.eqb_refl in Heval_orig.
+  simpl in Heval_orig.
+  destruct (eval_sstack_val' maxidx arg1 stk mem strg ctx idx sb evm_stack_opm)
+    as [arg1v|] eqn: eval_arg1; try discriminate.
+  destruct maxidx as [| maxidx']; try discriminate.
+  simpl in Heval_orig.
+  rewrite -> eq_follow_arg2 in Heval_orig.
+  simpl in Heval_orig.
+  destruct (eval_sstack_val' maxidx' arg21 stk mem strg ctx idx' sb' 
+    evm_stack_opm) as [arg21v|] eqn: eval_arg21; try discriminate.
+  destruct (eval_sstack_val' maxidx' arg22 stk mem strg ctx idx' sb' 
+    evm_stack_opm) as [arg22v|] eqn: eval_arg22; try discriminate.
+  
+  destruct (fcmp arg1 arg21 idx sb idx' sb' instk_height evm_stack_opm) 
+    eqn: eq_fcmp_arg1_arg21. 
+  + rewrite <- Heval_orig.
+    simpl.
+    injection Hoptm_sbinding as eq_val' _.
+    rewrite <- eq_val'.
+    unfold eval_sstack_val.
+    rewrite -> eval_sstack_val'_one_step. 
+    rewrite -> follow_in_smap_head_op.
+    rewrite -> evm_stack_opm_AND. 
+    rewrite -> lenght2.
+    unfold map_option.
+    rewrite -> eval_arg1.
+    rewrite -> eval'_maxidx_indep_eq with (m:=idx) in eval_arg22.
+    apply eval_sstack_val'_preserved_when_depth_extended in eval_arg22.
+    pose proof (follow_suffix sb arg2 idx (SymOp AND [arg21; arg22]) idx' sb'
+      eq_follow_arg2) as Hprefix_sb.
+    destruct Hprefix_sb as [prefix Hprefix_sb].
+    simpl in Hvalid.
+    destruct Hvalid as [eq_idx [Hvalid_stack_op Hvalid_sb]].    
+    pose proof (eval_sstack_val'_extend_sb instk_height (S maxidx') stk
+      mem strg ctx idx sb sb' evm_stack_opm prefix Hvalid_sb Hprefix_sb
+      arg22 arg22v eval_arg22) as Heval_arg22_sb.
+    rewrite -> Heval_arg22_sb. simpl.
+    
+    unfold valid_stack_op_instr in Hvalid_stack_op. simpl in Hvalid_stack_op.
+    destruct Hvalid_stack_op as [_ [Hvalid_arg1 [Hvalid_arg2 _]]].
+    pose proof (valid_follow_in_smap sb arg2 instk_height idx evm_stack_opm
+      (SymOp AND [arg21; arg22]) idx' sb' Hvalid_arg2 Hvalid_sb
+      eq_follow_arg2) as Hvalid2.
+    destruct Hvalid2 as [Hvalid_smapv_and [Hvalid_sb' Himpl]].
+    simpl in Hvalid_smapv_and. unfold valid_stack_op_instr in Hvalid_smapv_and.
+    simpl in Hvalid_smapv_and.
+    destruct Hvalid_smapv_and as [_ [valid_arg21 [valid_arg22 _]]].
+     
+    symmetry in Hlen.
+    pose proof (Hsafe_sstack_val_cmp arg1 arg21 idx sb idx' sb' instk_height 
+      evm_stack_opm Hvalid_arg1 valid_arg21 Hvalid_sb Hvalid_sb'
+      eq_fcmp_arg1_arg21 stk mem strg ctx Hlen) as Hcmp_eval.
+    destruct Hcmp_eval as [vv [eval_arg1_vv eval_arg21_vv]].
+    
+    injection eq_idx as eq_idx.
+    unfold eval_sstack_val in eval_arg1_vv.
+    unfold eval_sstack_val in eval_arg21_vv.
+    rewrite <- eq_idx in eval_arg1_vv. rewrite <- eq_idx in eval_arg1.
+    rewrite -> eval_arg1 in eval_arg1_vv.
+    pose proof (not_basic_value_smv_symop AND [arg21;arg22]) as not_basic_and.
+    apply Himpl in not_basic_and.
+    rewrite -> eq_idx in eval_arg21.
+    assert (S idx' <= idx) as Hleq.
+    * intuition.
+    * pose proof (eval_sstack_val'_preserved_when_depth_extended_le (S idx') 
+        idx idx' sb' arg21 vv stk mem strg ctx evm_stack_opm Hleq
+        eval_arg21_vv) as eval_arg21'.
+      rewrite -> eval_arg21 in eval_arg21'.
+      rewrite <- eval_arg1_vv in eval_arg21'.
+      injection eval_arg21' as eq_arg21v_arg1v.
+      rewrite -> eq_arg21v_arg1v.
+      rewrite -> wand_wand1_1.
+      reflexivity.
+
+  + destruct (fcmp arg1 arg22 idx sb idx' sb' instk_height evm_stack_opm)
+      eqn: eq_fcmp_arg1_arg22; try inject_rw Hoptm_sbinding eq_val'.
+    rewrite <- Heval_orig.
+    simpl.
+    injection Hoptm_sbinding as eq_val' _.
+    rewrite <- eq_val'.
+    unfold eval_sstack_val.
+    rewrite -> eval_sstack_val'_one_step. 
+    rewrite -> follow_in_smap_head_op.
+    rewrite -> evm_stack_opm_AND. 
+    rewrite -> lenght2.
+    unfold map_option.
+    rewrite -> eval_arg1.
+    rewrite -> eval'_maxidx_indep_eq with (m:=idx) in eval_arg21.
+    apply eval_sstack_val'_preserved_when_depth_extended in eval_arg21.
+    pose proof (follow_suffix sb arg2 idx (SymOp AND [arg21; arg22]) idx' sb'
+      eq_follow_arg2) as Hprefix_sb.
+    destruct Hprefix_sb as [prefix Hprefix_sb].
+    simpl in Hvalid.
+    destruct Hvalid as [eq_idx [Hvalid_stack_op Hvalid_sb]].
+    pose proof (eval_sstack_val'_extend_sb instk_height (S maxidx') stk
+      mem strg ctx idx sb sb' evm_stack_opm prefix Hvalid_sb Hprefix_sb
+      arg21 arg21v eval_arg21) as Heval_arg21_sb.
+    rewrite -> Heval_arg21_sb. simpl.
+    
+    unfold valid_stack_op_instr in Hvalid_stack_op. simpl in Hvalid_stack_op.
+    destruct Hvalid_stack_op as [_ [Hvalid_arg1 [Hvalid_arg2 _]]].
+    pose proof (valid_follow_in_smap sb arg2 instk_height idx evm_stack_opm
+      (SymOp AND [arg21; arg22]) idx' sb' Hvalid_arg2 Hvalid_sb
+      eq_follow_arg2) as Hvalid2.
+    destruct Hvalid2 as [Hvalid_smapv_and [Hvalid_sb' Himpl]].
+    simpl in Hvalid_smapv_and. unfold valid_stack_op_instr in Hvalid_smapv_and.
+    simpl in Hvalid_smapv_and.
+    destruct Hvalid_smapv_and as [_ [valid_arg21 [valid_arg22 _]]].
+
+    symmetry in Hlen.
+    pose proof (Hsafe_sstack_val_cmp arg1 arg22 idx sb idx' sb' instk_height 
+      evm_stack_opm Hvalid_arg1 valid_arg22 Hvalid_sb Hvalid_sb'
+      eq_fcmp_arg1_arg22 stk mem strg ctx Hlen) as Hcmp_eval.
+    destruct Hcmp_eval as [vv [eval_arg1_vv eval_arg22_vv]].
+    
+    injection eq_idx as eq_idx.
+    unfold eval_sstack_val in eval_arg1_vv.
+    unfold eval_sstack_val in eval_arg22_vv.
+    rewrite <- eq_idx in eval_arg1_vv. rewrite <- eq_idx in eval_arg1.
+    rewrite -> eval_arg1 in eval_arg1_vv.
+    pose proof (not_basic_value_smv_symop AND [arg21;arg22]) as not_basic_and.
+    apply Himpl in not_basic_and.
+    rewrite -> eq_idx in eval_arg22.
+    assert (S idx' <= idx) as Hleq.
+    * intuition.
+    * pose proof (eval_sstack_val'_preserved_when_depth_extended_le (S idx') 
+        idx idx' sb' arg22 vv stk mem strg ctx evm_stack_opm Hleq
+        eval_arg22_vv) as eval_arg22'.
+      rewrite -> eval_arg22 in eval_arg22'.
+      rewrite <- eval_arg1_vv in eval_arg22'.
+      injection eval_arg22' as eq_arg22v_arg1v.
+      rewrite -> eq_arg22v_arg1v.
+      rewrite <- wand_wand1_2.
+      reflexivity.
+Qed.
+
+End Opt_and_and1.
